src/simple_log_parser.ml
@@ -1,0 +1,159 @@
+(*
+ * This file is part of MONPOLY.
+ *
+ * Copyright (C) 2021 ETH Zurich.
+ *
+ * This library is free software; you can redistribute it and/or
+ * modify it under the terms of the GNU Lesser General Public License
+ * as published by the Free Software Foundation, version 2.1 of the
+ * License.
+ *
+ * This library is distributed in the hope that it will be useful, but
+ * WITHOUT ANY WARRANTY; without even the implied warranty of
+ * MERCHANTABILITY or FITNESS FOR A PARTICULAR PURPOSE. See the GNU
+ * Lesser General Public License for more details.
+ *
+ * You should have received a copy of the GNU Lesser General Public
+ * License along with this library. If not, see
+ * http://www.gnu.org/licenses/lgpl-2.1.html.
+ *
+ * As a special exception to the GNU Lesser General Public License,
+ * you may link, statically or dynamically, a "work that uses the
+ * Library" with a publicly distributed version of the Library to
+ * produce an executable file containing portions of the Library, and
+ * distribute that executable file under terms of your choice, without
+ * any of the additional requirements listed in clause 6 of the GNU
+ * Lesser General Public License. By "a publicly distributed version
+ * of the Library", we mean either the unmodified Library as
+ * distributed by Nokia, or a modified version of the Library that is
+ * distributed under the conditions defined in clause 3 of the GNU
+ * Lesser General Public License. This exception does not however
+ * invalidate any other reasons why the executable file might be
+ * covered by the GNU Lesser General Public License.
+ *)
+
+type token = Log_parser.token
+
+exception Stop_parser
+
+module type Consumer = sig
+  type ctxt
+  val begin_tp: ctxt -> MFOTL.timestamp -> unit
+  val observe: ctxt -> string -> Tuple.tuple -> unit
+  val end_tp: ctxt -> unit
+end
+
+type parsebuf = {
+  pb_lexbuf: Lexing.lexbuf;
+  mutable pb_token: token;
+  mutable pb_cur_rel: string;
+  mutable pb_cur_schema: (string * Predicate.tcst) list;
+  mutable pb_cur_ar: int;
+}
+
+let init_parsebuf lexbuf = {
+  pb_lexbuf = lexbuf;
+  pb_token = Log_lexer.token lexbuf;
+  pb_cur_rel = "";
+  pb_cur_schema = [];
+  pb_cur_ar = 0;
+}
+
+let next pb = pb.pb_token <- Log_lexer.token pb.pb_lexbuf
+
+let str_of_token = Log_parser.(function
+  | AT -> "AT"
+  | LPA -> "LPA"
+  | RPA -> "RPA"
+  | LCB -> "LCB"
+  | RCB -> "RCB"
+  | COM -> "COM"
+  | SEP -> "SEP"
+  | STR s -> "STR(" ^ s ^ ")"
+  | EOF -> "EOF"
+  | CMD -> "CMD"
+  | EOC -> "EOC"
+  | ERR -> "ERR")
+
+module Make(C: Consumer) = struct
+  let parse dbs lexbuf ctxt =
+    let pb = init_parsebuf lexbuf in
+    let fail () = failwith "[Simple_log_parser] Parse error" in
+    let process_tuple t =
+      if List.length t = pb.pb_cur_ar then
+        let t = try Tuple.make_tuple2 t pb.pb_cur_schema
+          with Tuple.Type_error str_err -> fail () in
+        C.observe ctxt pb.pb_cur_rel t
+      else
+        fail ()
+    in
+    let debug msg =
+      if Misc.debugging Misc.Dbg_log then
+        Printf.eprintf "[Simple_log_parser] %s with token=%s\n" msg
+          (str_of_token pb.pb_token)
+      else ()
+    in
+    let rec parse_init () =
+      debug "init";
+      match pb.pb_token with
+      | EOF -> ()
+      | AT -> next pb; parse_ts ()
+      | _ -> fail ()
+    and parse_ts () =
+      debug "ts";
+      match pb.pb_token with
+      | STR s ->
+          next pb;
+          C.begin_tp ctxt (MFOTL.ts_of_string "Simple_log_parser" s);
+          parse_db ()
+      | _ -> fail ()
+    and parse_db () =
+      debug "db";
+      match pb.pb_token with
+      | STR s ->
+          next pb;
+          pb.pb_cur_rel <- s;
+          pb.pb_cur_schema <- (try List.assoc s dbs with Not_found -> fail ());
+          pb.pb_cur_ar <- List.length pb.pb_cur_schema;
+          (match pb.pb_token with
+          | LPA -> next pb; parse_tuple ()
+          | _ -> process_tuple []; parse_db ())
+      | AT ->
+          next pb;
+          C.end_tp ctxt;
+          parse_ts ()
+      | SEP ->
+          next pb;
+          C.end_tp ctxt;
+          parse_init ()
+      | EOF -> C.end_tp ctxt
+      | _ -> fail ()
+    and parse_tuple () =
+      debug "tuple";
+      match pb.pb_token with
+      | RPA ->
+          next pb;
+          process_tuple [];
+          parse_db ()
+      | STR s ->
+          next pb;
+          parse_tuple_cont [s]
+      | _ -> fail ()
+    and parse_tuple_cont l =
+      debug "tuple_cont";
+      match pb.pb_token with
+      | RPA ->
+          next pb;
+          process_tuple (List.rev l);
+          parse_db ()
+      | COM ->
+          next pb;
+          (match pb.pb_token with
+          | STR s ->
+              next pb;
+              parse_tuple_cont (s::l)
+          | _ -> fail ())
+      | _ -> fail ()
+    in
+    try parse_init (); true with Stop_parser -> false
+end
