src/simple_log_parser.mli
@@ -1,0 +1,46 @@
+(*
+ * This file is part of MONPOLY.
+ *
+ * Copyright (C) 2021 ETH Zurich.
+ *
+ * This library is free software; you can redistribute it and/or
+ * modify it under the terms of the GNU Lesser General Public License
+ * as published by the Free Software Foundation, version 2.1 of the
+ * License.
+ *
+ * This library is distributed in the hope that it will be useful, but
+ * WITHOUT ANY WARRANTY; without even the implied warranty of
+ * MERCHANTABILITY or FITNESS FOR A PARTICULAR PURPOSE. See the GNU
+ * Lesser General Public License for more details.
+ *
+ * You should have received a copy of the GNU Lesser General Public
+ * License along with this library. If not, see
+ * http://www.gnu.org/licenses/lgpl-2.1.html.
+ *
+ * As a special exception to the GNU Lesser General Public License,
+ * you may link, statically or dynamically, a "work that uses the
+ * Library" with a publicly distributed version of the Library to
+ * produce an executable file containing portions of the Library, and
+ * distribute that executable file under terms of your choice, without
+ * any of the additional requirements listed in clause 6 of the GNU
+ * Lesser General Public License. By "a publicly distributed version
+ * of the Library", we mean either the unmodified Library as
+ * distributed by Nokia, or a modified version of the Library that is
+ * distributed under the conditions defined in clause 3 of the GNU
+ * Lesser General Public License. This exception does not however
+ * invalidate any other reasons why the executable file might be
+ * covered by the GNU Lesser General Public License.
+ *)
+
+exception Stop_parser
+
+module type Consumer = sig
+  type ctxt
+  val begin_tp: ctxt -> MFOTL.timestamp -> unit
+  val observe: ctxt -> string -> Predicate.cst list -> unit
+  val end_tp: ctxt -> unit
+end
+
+module Make(C: Consumer): sig
+  val parse: Db.schema -> Lexing.lexbuf -> C.ctxt -> bool
+end
