src/verified_adapter.ml
@@ -79,6 +79,15 @@ let convert_agg_op = function
   | Avg -> Agg_Avg
   | Med -> Agg_Med
 
+(* These must be synchronized with Log.get_signature_lexbuf *)
+let special_predicates = ["tp"; "ts"; "tpts"]
+
+let convert_special_predicate fvl bvl = function
+  | ("tp", _, [t]) -> TP (convert_term fvl bvl t)
+  | ("ts", _, [t]) -> TS (convert_term fvl bvl t)
+  | ("tpts", _, [t1; t2]) -> And (TP (convert_term fvl bvl t1), TS (convert_term fvl bvl t2))
+  | _ -> failwith "[convert_special_predicate] internal error"
+
 let convert_formula dbschema f =
   let free_vars = MFOTL.free_vars f in
   let truth = Equal (Cst (Int 0), Cst (Int 0)) in
@@ -86,26 +95,33 @@ let convert_formula dbschema f =
   | 0 -> f
   | n -> createExists (n-1) (Exists f)
   in
-  let rec convert_formula_vars fvl bvl = function
+  let rec convert_formula_vars fvl bvl lets = function
   | Equal (t1,t2) -> Eq (convert_term fvl bvl t1, convert_term fvl bvl t2)
   | Less (t1,t2) -> Less (convert_term fvl bvl t1, convert_term fvl bvl t2)
   | LessEq (t1,t2) -> LessEq (convert_term fvl bvl t1, convert_term fvl bvl t2)
-  | Pred (p,_,tl) -> Pred (p, List.map (fun t -> convert_term fvl bvl t) tl)
+  | Pred p ->
+      let (n, a, tl) = p in
+      if List.mem n special_predicates && not (List.mem (n, a) lets) then
+        convert_special_predicate fvl bvl p
+      else
+        Pred (n, List.map (convert_term fvl bvl) tl)
   | Let (p,f1,f2) ->
       let (n,a,ts) = Predicate.get_info p in
       let fvl1 = List.flatten (List.map Predicate.tvars ts) in
-      Let (n, convert_formula_vars fvl1 [] f1, convert_formula_vars fvl bvl f2)
+      let lets2 = (n, a) :: lets in
+      Let (n, convert_formula_vars fvl1 [] lets f1, convert_formula_vars fvl bvl lets2 f2)
   | LetPast (p,f1,f2) ->
       let (n,a,ts) = Predicate.get_info p in
       let fvl1 = List.flatten (List.map Predicate.tvars ts) in
-      LetPast (n, convert_formula_vars fvl1 [] f1, convert_formula_vars fvl bvl f2)
-  | Neg f -> Neg (convert_formula_vars fvl bvl f)
-  | And (f1,f2) -> And (convert_formula_vars fvl bvl f1, convert_formula_vars fvl bvl f2)
-  | Or (f1,f2) -> Or (convert_formula_vars fvl bvl f1, convert_formula_vars fvl bvl f2)
-  | Implies (f1,f2) -> convert_formula_vars fvl bvl (Or ((Neg f1), f2))
-  | Equiv (f1,f2) -> convert_formula_vars fvl bvl (And (Implies (f1,f2),Implies(f2,f2)))
-  | Exists (v,f) -> createExists (List.length v) (convert_formula_vars fvl (v@bvl) f)
-  | ForAll (v,f) -> convert_formula_vars fvl bvl (Neg (Exists (v,(Neg f))))
+      let lets' = (n, a) :: lets in
+      LetPast (n, convert_formula_vars fvl1 [] lets' f1, convert_formula_vars fvl bvl lets' f2)
+  | Neg f -> Neg (convert_formula_vars fvl bvl lets f)
+  | And (f1,f2) -> And (convert_formula_vars fvl bvl lets f1, convert_formula_vars fvl bvl lets f2)
+  | Or (f1,f2) -> Or (convert_formula_vars fvl bvl lets f1, convert_formula_vars fvl bvl lets f2)
+  | Implies (f1,f2) -> convert_formula_vars fvl bvl lets (Or ((Neg f1), f2))
+  | Equiv (f1,f2) -> convert_formula_vars fvl bvl lets (And (Implies (f1,f2),Implies(f2,f2)))
+  | Exists (v,f) -> createExists (List.length v) (convert_formula_vars fvl (v@bvl) lets f)
+  | ForAll (v,f) -> convert_formula_vars fvl bvl lets (Neg (Exists (v,(Neg f))))
   | Aggreg (t_y, y,op,x,glist,f) ->
       let t_y = match t_y with TCst a -> a | _ -> failwith "Internal error" in
       let attr = MFOTL.free_vars f in
@@ -115,51 +131,58 @@ let convert_formula dbschema f =
         (convert_agg_op op, convert_cst (aggreg_default_value op t_y)),
         nat_of_int (List.length bound),
         convert_term fvl bvl_f (Var x),
-        convert_formula_vars fvl bvl_f f)
-  | Prev (intv,f) -> Prev ((convert_interval intv), (convert_formula_vars fvl bvl f))
-  | Next (intv,f) -> Next ((convert_interval intv), (convert_formula_vars fvl bvl f))
-  | Since (intv,f1,f2) -> Since (convert_formula_vars fvl bvl f1,convert_interval intv,convert_formula_vars fvl bvl f2)
-  | Until (intv,f1,f2) -> Until (convert_formula_vars fvl bvl f1,convert_interval intv,convert_formula_vars fvl bvl f2)
-  | Eventually (intv,f) -> convert_formula_vars fvl bvl (Until (intv,truth,f))
-  | Once (intv,f) -> convert_formula_vars fvl bvl (Since (intv,truth,f))
-  | Always (intv,f) -> convert_formula_vars fvl bvl (Neg (Eventually (intv,(Neg f))))
-  | PastAlways (intv,f) -> convert_formula_vars fvl bvl (Neg (Once (intv,(Neg f))))
-  | Frex (intv, r) -> MatchF (convert_interval intv, convert_re_vars fvl bvl r)
-  | Prex (intv, r) -> MatchP (convert_interval intv, convert_re_vars fvl bvl r)
+        convert_formula_vars fvl bvl_f lets f)
+  | Prev (intv,f) -> Prev ((convert_interval intv), (convert_formula_vars fvl bvl lets f))
+  | Next (intv,f) -> Next ((convert_interval intv), (convert_formula_vars fvl bvl lets f))
+  | Since (intv,f1,f2) -> Since (convert_formula_vars fvl bvl lets f1,convert_interval intv,convert_formula_vars fvl bvl lets f2)
+  | Until (intv,f1,f2) -> Until (convert_formula_vars fvl bvl lets f1,convert_interval intv,convert_formula_vars fvl bvl lets f2)
+  | Eventually (intv,f) -> convert_formula_vars fvl bvl lets (Until (intv,truth,f))
+  | Once (intv,f) -> convert_formula_vars fvl bvl lets (Since (intv,truth,f))
+  | Always (intv,f) -> convert_formula_vars fvl bvl lets (Neg (Eventually (intv,(Neg f))))
+  | PastAlways (intv,f) -> convert_formula_vars fvl bvl lets (Neg (Once (intv,(Neg f))))
+  | Frex (intv, r) -> MatchF (convert_interval intv, convert_re_vars fvl bvl lets r)
+  | Prex (intv, r) -> MatchP (convert_interval intv, convert_re_vars fvl bvl lets r)
   | _ -> failwith "[convert_term] unsupported formula"
-and convert_re_vars fvl bvl = function
+and convert_re_vars fvl bvl lets = function
   | Wild -> wild
-  | Test f -> Test (convert_formula_vars fvl bvl f)
-  | Concat (r1,r2) -> Times (convert_re_vars fvl bvl r1, convert_re_vars fvl bvl r2)
-  | Plus (r1,r2) -> Plusa (convert_re_vars fvl bvl r1, convert_re_vars fvl bvl r2)
-  | Star r -> Star (convert_re_vars fvl bvl r)
-  in convert_formula_vars free_vars [] f
+  | Test f -> Test (convert_formula_vars fvl bvl lets f)
+  | Concat (r1,r2) -> Times (convert_re_vars fvl bvl lets r1, convert_re_vars fvl bvl lets r2)
+  | Plus (r1,r2) -> Plusa (convert_re_vars fvl bvl lets r1, convert_re_vars fvl bvl lets r2)
+  | Star r -> Star (convert_re_vars fvl bvl lets r)
+  in convert_formula_vars free_vars [] [] f
 
-let unorderedFlatMap m =
-  let rec flatmap_rec acc = function
-  | [] -> acc
-  | x::xs -> flatmap_rec (List.rev_append (m x) acc) xs in
-  flatmap_rec []
+type state =
+  (((nat *
+      (nat *
+        (bool list *
+          (bool list *
+            ((nat * ((event_data option) list) set) queue *
+              ((nat * ((event_data option) list) set) queue *
+                (((event_data option) list) set *
+                  ((((event_data option) list), nat) mapping *
+                    (((event_data option) list), nat) mapping)))))))) *
+     aggaux option),
+    ((nat *
+       (nat queue *
+         ((((event_data option) list) set * (nat, nat) sum) queue *
+           (nat *
+             (bool list *
+               (bool list *
+                 (((event_data option) list) set *
+                   ((((event_data option) list), nat) mapping *
+                     ((nat, (((event_data option) list), (nat, nat) sum)
+                              mapping)
+                        mapping *
+                       ((nat, nat) mapping *
+                         (((event_data option) list) set list *
+                           nat))))))))))) *
+      aggaux option),
+    unit)
+    mistate_ext
 
-let convert_db md =
-  let rbt_single x = RBT_set (rbt_insert x rbt_empty) in
-  let convert_cst' x = Some (convert_cst x) in
-  let add_builtin xs (name, tup) =
-    let arity = nat_of_int (List.length tup) in
-    ((name, arity), rbt_single (List.map convert_cst' tup)) :: xs
-  in
-  let convert_table t =
-    let (name, attrs) = (Table.get_schema t) in
-    let arity = nat_of_int (List.length attrs) in
-    ((name, arity), RBT_set (Relation.fold
-      (fun v -> rbt_insert (List.map convert_cst' v))
-      (Table.get_relation t) rbt_empty))
-  in
-  let db_events = List.map convert_table (Db.get_tables md.db) in
-  let all_events = List.fold_left add_builtin db_events
-    ["tp", [Int md.tp]; "ts", [Float md.ts]; "tpts", [Int md.tp; Float md.ts]]
-  in
-  (mk_db all_events, nat_of_float md.ts)
+let init cf = minit_incr cf
+
+let observe e t st = mobserve e (List.map convert_cst t) st
 
 let cst_of_event_data = function
   | EInt x -> (try Int (Z.to_int x) with Z.Overflow -> ZInt x)
@@ -177,6 +200,10 @@ let convert_violations =
     ((int_of_nat tp),
      Relation.make_relation
       (rbt_fold (fun t l -> (convert_tuple t) :: l) v [] )))
+
+let conclude ts st =
+  let (vs, st') = mconclude (nat_of_float ts) st in
+  (convert_violations vs, st')
 
 let is_monitorable dbschema f =
   let s = (mmonitorable_exec << convert_formula dbschema) f in
