src/verified_adapter.mli
@@ -5,7 +5,8 @@ open Helper
 
 val is_monitorable: Db.schema -> formula -> bool * (formula * string) option
 val convert_formula: Db.schema -> formula -> Verified.Monitor.formula
-val convert_db: monpolyData -> (string * Verified.Monitor.nat,
-  Verified.Monitor.event_data option list Verified.Monitor.set list) Verified.Monitor.mapping *
-  Verified.Monitor.nat
-val convert_violations: (Verified.Monitor.nat * Verified.Monitor.event_data option list Verified.Monitor.set) list -> (int * relation) list
+
+type state
+val init: Verified.Monitor.formula -> state
+val observe: string -> cst list -> state -> state
+val conclude: timestamp -> state -> (int * relation) list * state
